examples/test_inductive_principle.v
@@ -124,7 +124,124 @@ Print indp_acc.
   non-uniform parameter,
 
   Notice that the (type of) uniform parameter cannot depend on the non-uniform parameters.
-
-
-
 *)
+
+
+
+
+
+
+
+(* Load MetaCoqPrelude.
+Definition thisfile := $run (tmCurrentModPath tt).
+Definition input := ($run (tmQuoteInductive (thisfile, "myt"))).
+Print input. *)
+(* MetaCoq Run PrintInductivePrinciple myt. *)
+(* MetaCoq Run Derive InductivePrinciple myt as "indp_myt".
+Print indp_myt. *)
+
+(* strange test case *)
+Inductive myt0 (A:Type) (B: Type) : Type :=
+  | Build0 (x:A) (b:B) (c:
+    (fun x => match x with
+    | 0 => A
+    | _ => A end) (3)
+  ).
+MetaCoq Run Derive InductivePrinciple myt0 as "indp_myt0".
+Print indp_myt0.
+
+
+Inductive myt (A:Type) (B: Type) : Type :=
+  | Build (x:A) (b:B) (c:
+    (let fix f x :=
+      match x with
+      | 0 => A
+      | S n' => f n' end in f 3
+    )
+  ).
+MetaCoq Run Derive InductivePrinciple myt as "indp_myt".
+Print indp_myt.
+
+
+Inductive myt1 (A:Type) (B: Type) : Type :=
+  | Build1 (x:A) (b:B) (c:let x:= A in prod x B).
+MetaCoq Run Derive InductivePrinciple myt1 as "indp_myt1".
+Print indp_myt1.
+
+
+
+Inductive testletin : let x := nat in x -> Type :=
+  | C0: (let x := nat in x) -> (let y := option nat in prod y y ->
+          nat) -> let z := nat in let w := z in w -> testletin 0.
+MetaCoq Run Derive InductivePrinciple testletin as "indp_testletin".
+Print indp_testletin.
+(*
+forall P : testletin -> Prop,
+       (forall (p : let x := nat in x)
+          (n : let y := option nat in y * y -> nat),
+        let z := nat in let w := z in forall w0 : w, P (C0 p n w0)) ->
+       forall t : testletin, P t
+*)
+(* MetaCoq Run PrintInductivePrinciple testletin. *)
+
+(* Load MetaCoqPrelude.
+Definition thisfile := $run (tmCurrentModPath tt).
+Definition input := ($run (tmQuoteInductive (thisfile, "testletin"))).
+Print input.
+
+Print testletin_ind. *)
+
+(* Compute $quote (forall P : let x := nat in testletin -> Prop,
+(forall (p : let x := nat in x)
+   (n : let y := option nat in y × y -> nat),
+ let z := nat in let w := z in forall w0 : w, P (C0 p n w0)) ->
+forall t : testletin, P t). *)
+
+
+
+(* Print input.
+Print indp_testletin.
+MetaCoq Run PrintInductivePrinciple testletin. *)
+
+
+Inductive mynat'' :Type :=
+  | myz''
+  | mys'' : let x := mynat'' in mynat'' -> mynat''.
+
+MetaCoq Run Derive InductivePrinciple mynat'' as "indp_mynat''".
+Print indp_mynat''.
+
+(* Load MetaCoqPrelude.
+Definition thisfile := $run (tmCurrentModPath tt).
+Definition input := ($run (tmQuoteInductive (thisfile, "mynat'"))).
+Print input. *)
+
+Inductive myvec' (A:Type) : let x := nat in x -> Type :=
+  | myvnil' : myvec' A 0
+  | myvcons' : let a := A in a -> forall n, let z := myvec' in z a n -> myvec' A (S n).
+MetaCoq Run Derive InductivePrinciple myvec' as "indp_myvec'".
+Print indp_myvec'.
+
+(* Load MetaCoqPrelude.
+Definition thisfile := $run (tmCurrentModPath tt).
+Definition input := ($run (tmQuoteInductive (thisfile, "myvec'"))).
+Print input. *)
+
+(* Compute  *)
+
+
+
+Inductive mynat' :Type :=
+  | myz'
+  | mys' : let x := mynat' in let y := x in ((fun z => z ) y) -> mynat'.
+
+(* MetaCoq Run PrintInductivePrinciple mynat'. *)
+
+(* Load MetaCoqPrelude.
+Definition thisfile := $run (tmCurrentModPath tt).
+Definition input := ($run (tmQuoteInductive (thisfile, "mynat'"))).
+Print input. *)
+
+
+MetaCoq Run Derive InductivePrinciple mynat' as "indp_mynat'".
+Print indp_mynat'.
